theories/Prelude.v
@@ -1,0 +1,6 @@
+From stdpp Require Export prelude.
+
+From RSL Require Export Prelude.Definitions.
+From RSL Require Export Prelude.Language.
+From RSL Require Export Prelude.Utils.
+From RSL Require Export Prelude.NoDup.
