theories/Toy/Compile.v
@@ -1,4 +1,4 @@
-From stdpp Require Import prelude.
+From RSL Require Import Prelude.
 
 From RSL Require Import RTL.RTL.
 From RSL Require Import Toy.Toy.
